extraction/theories/ErasureTests.v
@@ -1,0 +1,270 @@
+From ConCert.Extraction Require Import Erasure.
+From ConCert.Extraction Require Import ResultMonad.
+From ConCert.Extraction Require Import StringExtra.
+From Coq Require Import Ascii.
+From Coq Require Import Bool.
+From Coq Require Import List.
+From Coq Require Import String.
+From MetaCoq.Erasure Require Import SafeTemplateErasure.
+From MetaCoq.PCUIC Require Import PCUICAst.
+From MetaCoq.PCUIC Require Import PCUICTyping.
+From MetaCoq.PCUIC Require Import TemplateToPCUIC.
+From MetaCoq.SafeChecker Require Import PCUICSafeChecker.
+From MetaCoq.SafeChecker Require Import SafeTemplateChecker.
+From MetaCoq.Template Require Import Loader.
+From MetaCoq.Template Require Import config.
+From MetaCoq.Template Require Import monad_utils.
+From MetaCoq.Template Require Import utils.
+
+Local Open Scope string_scope.
+Import ListNotations.
+Import MonadNotation.
+Set Equations Transparent.
+
+Module E := MetaCoq.Erasure.EAst.
+
+Module flag_of_type_tests.
+Record type_flag_squashed := {
+  is_logical : bool;
+  is_sort : bool;
+  is_arity : bool }.
+
+Program Definition flag_of_type_program (p : Ast.program)
+  : result type_flag_squashed string :=
+  let Σ := List.rev (trans_global (Ast.empty_ext p.1)).1 in
+  G <- match check_wf_env_only_univs Σ with
+       | CorrectDecl a => ret a
+       | _ => Err "Could not check_wf_env_only_univs"
+       end;;
+  f <- match flag_of_type (empty_ext Σ) _ [] (trans p.2) _ with
+       | Checked a => ret a
+       | TypeError te => Err "Could not get flag"
+       end;;
+  ret {| is_logical := Erasure.is_logical f;
+         is_sort := if Erasure.is_sort f then true else false;
+         is_arity := if Erasure.is_arity f then true else false |}.
+Next Obligation.
+  unfold trans_global.
+  simpl. unfold wf_ext, empty_ext. simpl.
+  unfold on_global_env_ext. destruct H0. constructor.
+  split; auto. simpl. todo "on_udecl on empty universe context".
+Qed.
+Next Obligation.
+  unfold trans_global.
+  simpl. unfold wf_ext, empty_ext. simpl.
+  unfold on_global_env_ext. destruct H0. todo "assuming well-typedness".
+Qed.
+
+Quote Recursively Definition ex1 := Type.
+Check eq_refl : ltac:(let x := eval vm_compute in (flag_of_type_program ex1) in exact x) =
+                Ok {| is_logical := false; is_sort := true; is_arity := true |}.
+
+Quote Recursively Definition ex2 := nat.
+Check eq_refl : ltac:(let x := eval vm_compute in (flag_of_type_program ex2) in exact x) =
+                Ok {| is_logical := false; is_sort := false; is_arity := false |}.
+
+Quote Recursively Definition ex3 := (nat -> nat).
+Check eq_refl : ltac:(let x := eval vm_compute in (flag_of_type_program ex3) in exact x) =
+                Ok {| is_logical := false; is_sort := false; is_arity := false |}.
+
+Quote Recursively Definition ex4 := (forall A, A).
+Check eq_refl : ltac:(let x := eval vm_compute in (flag_of_type_program ex4) in exact x) =
+                Ok {| is_logical := false; is_sort := false; is_arity := false |}.
+
+Quote Recursively Definition ex5 := (Prop).
+Check eq_refl : ltac:(let x := eval vm_compute in (flag_of_type_program ex5) in exact x) =
+                Ok {| is_logical := true; is_sort := true; is_arity := true |}.
+
+Quote Recursively Definition ex6 := (Prop -> Type).
+Check eq_refl : ltac:(let x := eval vm_compute in (flag_of_type_program ex6) in exact x) =
+                Ok {| is_logical := false; is_sort := false; is_arity := true |}.
+
+Quote Recursively Definition ex7 := (Type -> Prop).
+Check eq_refl : ltac:(let x := eval vm_compute in (flag_of_type_program ex7) in exact x) =
+                Ok {| is_logical := true; is_sort := false; is_arity := true |}.
+
+Quote Recursively Definition ex8 := (False).
+Check eq_refl : ltac:(let x := eval vm_compute in (flag_of_type_program ex8) in exact x) =
+                Ok {| is_logical := true; is_sort := false; is_arity := false |}.
+
+Quote Recursively Definition ex9 := (Fin.t 0 -> False).
+Check eq_refl : ltac:(let x := eval vm_compute in (flag_of_type_program ex9) in exact x) =
+                Ok {| is_logical := true; is_sort := false; is_arity := false |}.
+End flag_of_type_tests.
+
+Module erase_type_tests.
+Program Definition erase_type_program (p : Ast.program)
+  : result (EAst.global_context * (list name * box_type)) erase_type_error :=
+  let Σ := List.rev (trans_global (Ast.empty_ext p.1)).1 in
+  G <- match check_wf_env_only_univs Σ with
+       | CorrectDecl a => ret a
+       | _ => Err (GeneralError "Could not check_wf_env_only_univs")
+       end;;
+  Σ' <- wrap_typing_result (SafeErasureFunction.erase_global Σ _);;
+  t <- erase_type (empty_ext Σ) _ [] (Vector.nil _) (trans p.2) _ [];;
+  ret (Σ', t).
+Next Obligation.
+  unfold trans_global.
+  simpl. unfold wf_ext, empty_ext. simpl.
+  unfold on_global_env_ext. destruct H0. constructor.
+  split; auto. simpl. todo "on_udecl on empty universe context".
+Qed.
+Next Obligation.
+  unfold trans_global.
+  simpl. unfold wf_ext, empty_ext. simpl.
+  unfold on_global_env_ext. destruct H0. todo "assuming well-typedness".
+Qed.
+
+Definition is_arr (t : box_type) : bool :=
+  match t with
+  | TArr _ _ => true
+  | _ => false
+  end.
+
+Definition kername_unqual (name : kername) : string :=
+  match last_index_of "." name with
+  | Some n => substring_from (S n) name
+  | None => ""
+  end.
+
+Definition parenthesize_arg (a : box_type) : bool :=
+  match a with
+  | TBox
+  | TAny
+  | TVar _
+  | TInd _
+  | TConst _ => true
+  | _ => false
+  end.
+
+Fixpoint print_box_type (Σ : E.global_context) (bt : box_type) :=
+  match bt with
+  | TBox => "□"
+  | TAny => "𝕋"
+  | TArr dom codom => parens (negb (is_arr dom)) (print_box_type Σ dom) ++ " → " ++ print_box_type Σ codom
+  | TApp t1 t2 => print_box_type Σ t1 ++ " " ++ parens (parenthesize_arg t2) (print_box_type Σ t2)
+  | TVar i => "'a" ++ string_of_nat i
+  | TInd s =>
+    match EPretty.lookup_ind_decl Σ s.(inductive_mind) s.(inductive_ind) with
+    | Some oib => oib.(E.ind_name)
+    | None => "UndeclaredIductive(" ++ s.(inductive_mind)
+                                    ++ ","
+                                    ++ s.(inductive_mind)
+                                    ++ ")"
+    end
+  | TConst s => kername_unqual s
+  end.
+
+Definition print_type_vars (l : list name) :=
+  String.concat " " (map (fun na => match na with
+                                    | nAnon => "_"
+                                    | nNamed i => i
+                                    end) l).
+
+Definition erase_and_print_type
+           {cf : checker_flags}
+           (after_erasure : box_type -> box_type)
+           (p : Ast.program)
+  : result (string × string) erase_type_error :=
+  let p := fix_program_universes p in
+  '(Σ, (tvars, bt)) <- erase_type_program p;;
+  ret (print_type_vars tvars, print_box_type Σ bt).
+
+Quote Recursively Definition ex1 := (forall (A B : Type) (a : A * B) (C : Type), A * B * C).
+Check eq_refl : ltac:(let x := eval vm_compute in (erase_and_print_type id ex1) in exact x) =
+                Ok ("A B C", "□ → □ → prod 'a0 'a1 → □ → prod (prod 'a0 'a1) 'a2").
+
+Quote Recursively Definition ex2 := (forall (A : Type) (P : A -> Prop), @sig A P).
+Check eq_refl : ltac:(let x := eval vm_compute in (erase_and_print_type id ex2) in exact x) =
+                Ok ("A", "□ → □ → sig 'a0 □").
+
+Quote Recursively Definition ex3 := (forall (A : Type) (P : A -> Prop), { a : A | P a }).
+Check eq_refl : ltac:(let x := eval vm_compute in (erase_and_print_type id ex3) in exact x) =
+                Ok ("A", "□ → □ → sig 'a0 □").
+
+Quote Recursively Definition ex4 := (forall (A B : Type) (f : A -> B) (n : nat),
+                                        Vector.t A n -> Vector.t B n).
+Check eq_refl : ltac:(let x := eval vm_compute in (erase_and_print_type id ex4) in exact x) =
+                Ok ("A B", "□ → □ → ('a0 → 'a1) → nat → t 'a0 𝕋 → t 'a1 𝕋").
+
+Quote Recursively Definition ex5 :=
+  (forall (A : Type),  list A -> list A -> 0 = 0 -> forall (B : Type), B -> A -> A).
+Check eq_refl : ltac:(let x := eval vm_compute in (erase_and_print_type id ex5) in exact x) =
+                Ok ("A B", "□ → list 'a0 → list 'a0 → □ → □ → 'a1 → 'a0 → 'a0").
+
+(* Prenex form that we fail on *)
+Quote Recursively Definition ex6 :=
+  (forall (A : Type), (forall A : Type, A -> A) -> A -> forall B : Type, B -> nat).
+Check eq_refl : ltac:(let x := eval vm_compute in (erase_and_print_type id ex6) in exact x) =
+                Err NotPrenex.
+
+(** Erasing and deboxing *)
+Quote Recursively Definition ex7 :=
+  (forall (A : Type), A -> forall (B : Type) (C : Type), B -> C).
+Check eq_refl : ltac:(let x := eval vm_compute in (erase_and_print_type id ex7) in exact x) =
+                Ok ("A B C", "□ → 'a0 → □ → □ → 'a1 → 'a2").
+
+(** Tesing mutual inductives *)
+Inductive tree (A : Set) : Set :=
+  node : A -> forest A -> tree A
+with forest (A : Set) : Set :=
+    leaf : A -> forest A
+  | cons : tree A -> forest A -> forest A.
+
+Quote Recursively Definition ex8 := (forall (A: Set), forest A -> tree A -> A).
+Check eq_refl : ltac:(let x := eval vm_compute in (erase_and_print_type id ex8) in exact x) =
+                Ok ("A", "□ → forest 'a0 → tree 'a0 → 'a0").
+
+(* We cannot currently handle the following even though we may want to be able to.
+   To handle this we would need to do deboxing simultaneously with erasure. *)
+Quote Recursively Definition ex9 := (forall (A : 0 = 0 -> Type) (B : Type), option (A eq_refl) -> B).
+Check eq_refl : ltac:(let x := eval vm_compute in (erase_and_print_type id ex9) in exact x) =
+                Err NotPrenex.
+
+Quote Recursively Definition ex10 :=
+  (forall (A : Type), (forall (B : Type), B -> B) -> A).
+Check eq_refl : ltac:(let x := eval vm_compute in (erase_and_print_type id ex10) in exact x) =
+                Err NotPrenex.
+
+Definition non_neg := {n : nat | 0 < n}.
+
+Quote Recursively Definition ex11 := (forall (A : Type), {n : nat | 0 < n} -> A).
+Check eq_refl : ltac:(let x := eval vm_compute in (erase_and_print_type id ex11) in exact x) =
+                Ok ("A", "□ → sig nat □ → 'a0").
+
+Quote Recursively Definition ex12 := (forall (A : Type) (P : A -> Prop), unit).
+Check eq_refl : ltac:(let x := eval vm_compute in (erase_and_print_type id ex12) in exact x) =
+                Ok ("A", "□ → □ → unit").
+
+Quote Recursively Definition ex13 := (let p := (nat, unit) in fst p × snd p).
+Check eq_refl : ltac:(let x := eval vm_compute in (erase_and_print_type id ex13) in exact x) =
+                Ok ("", "prod (fst □ □ 𝕋) (snd □ □ 𝕋)").
+
+Quote Recursively Definition ex14 := (let t := nat in t).
+Check eq_refl : ltac:(let x := eval vm_compute in (erase_and_print_type id ex14) in exact x) =
+                Ok ("", "nat").
+
+Quote Recursively Definition ex15 := ((fix f n := match n with
+                                                  | 0 => nat
+                                                  | S n => nat -> f n
+                                                  end) 5).
+Check eq_refl : ltac:(let x := eval vm_compute in (erase_and_print_type id ex15) in exact x) =
+                Ok ("", "nat → nat → nat → nat → nat → nat").
+
+Quote Recursively Definition ex16 := (Type -> Type).
+Check eq_refl : ltac:(let x := eval vm_compute in (erase_and_print_type id ex16) in exact x) =
+                Ok ("_", "□ → □").
+
+Quote Recursively Definition ex17 := (Type -> Prop).
+Check eq_refl : ltac:(let x := eval vm_compute in (erase_and_print_type id ex17) in exact x) =
+                Ok ("", "□").
+
+Quote Recursively Definition ex18 := (False).
+Check eq_refl : ltac:(let x := eval vm_compute in (erase_and_print_type id ex18) in exact x) =
+                Ok ("", "□").
+
+Quote Recursively Definition ex19 := (Fin.t 0 -> False).
+Check eq_refl : ltac:(let x := eval vm_compute in (erase_and_print_type id ex19) in exact x) =
+                Ok ("", "□").
+
+End erase_type_tests.
